Started writing a reflective tactic for groups — it's not feature complete and doesn't work yet.

Instances/Setoid/Grp.v
@@ -20,6 +20,61 @@ Hint Resolve inv_l inv_r.
 
 Coercion mon : Grp >-> Mon.
 
+Theorem inv_involutive : forall (G : Grp) (g : G),
+    inv (inv g) == g.
+Proof.
+  intros. pose (@op_Proper G).
+  assert (op (inv (inv g)) (op (inv g) g) == g).
+    rewrite assoc, inv_l, neutr_l. reflexivity.
+    rewrite inv_l , neutr_r in H. assumption.
+Qed.
+
+Theorem neutr_unique_l : forall (G : Grp) (e : G),
+    (forall g : G, op e g == g) -> e == neutr.
+Proof.
+  intros.
+  assert (op e neutr == e). rewrite neutr_r. reflexivity.
+  assert (op e neutr == neutr). apply H.
+  rewrite H0 in H1. assumption.
+Defined.
+
+Theorem neutr_unique_r : forall (G : Grp) (e : G),
+    (forall g : G, op g e == g) -> e == neutr.
+Proof.
+  intros.
+  assert (op neutr e == e). rewrite neutr_l. reflexivity.
+  assert (op neutr e == neutr). apply H. 
+  rewrite H0 in H1. assumption.
+Defined.
+
+Theorem inv_op : forall (G : Grp) (a b : G),
+    inv (op a b) == op (inv b) (inv a).
+Proof.
+  intros. pose (@op_Proper G).
+  assert (forall x y : G, op (op x y) (inv (op x y)) == neutr). auto.
+  assert (forall x y : G, op (op x y) (op (inv y) (inv x)) == neutr).
+    intros. rewrite <- assoc. rewrite (assoc y _). rewrite inv_r.
+    rewrite neutr_l. auto.
+  assert (op (op a b) (inv (op a b)) == op (op a b) (op (inv b) (inv a))).
+    rewrite H, H0. reflexivity.
+  assert (op (inv (op a b)) (op (op a b) (inv (op a b))) ==
+    op (inv (op a b)) (op (op a b) (op (inv b) (inv a)))).
+    rewrite H1. reflexivity.
+  repeat rewrite assoc, inv_l, neutr_l in H2. assumption.
+Defined.
+
+Theorem inv_neutr : forall (G : Grp), inv neutr == neutr.
+Proof.
+  intros.
+  assert (op (inv neutr) neutr == neutr).
+    rewrite inv_l. reflexivity.
+  assert (op (inv neutr) neutr == inv neutr).
+    rewrite neutr_r. reflexivity.
+  rewrite <- H0, H. reflexivity.
+Defined.
+
+Hint Resolve inv_involutive neutr_unique_l neutr_unique_r inv_op inv_neutr.
+
 Ltac grp_simpl := simpl; intros;
 try match goal with
   (* There's a group that wasn't destructed. *)
@@ -93,6 +148,217 @@ Ltac grphoms' := grphoms_template grphom'.
 Ltac grp' := repeat (grp_simpl || grpobs' || grphoms' || mon').
 Ltac grp := try (grp'; fail).
 
+Inductive exp : Grp -> Type :=
+    | Id : forall X : Grp, exp X
+    | Var : forall X : Grp, X -> exp X
+    | Op : forall X : Grp, exp X -> exp X -> exp X
+    | Mor : forall X Y : Grp, GrpHom X Y -> exp X -> exp Y
+    | Inv : forall X : Grp, exp X -> exp X.
+
+Arguments Id [X].
+Arguments Var [X] _.
+Arguments Op [X] _ _.
+Arguments Mor [X Y] _ _ .
+Arguments Inv [X] _.
+
+(*Inductive exp (X : Grp) : Type :=
+    | Id : exp X
+    | Var : X -> exp X
+    | Op : exp X -> exp X -> exp X
+    | Mor : forall A : Grp, GrpHom A X -> exp A -> exp X
+    | Inv : exp X -> exp X.
+
+Arguments Id [X].
+Arguments Var [X] _.
+Arguments Op [X] _ _.
+Arguments Mor [X A] _ _.
+Arguments Inv [X] _.
+*)
+
+Fixpoint expDenote {X : Grp} (e : exp X) : X :=
+match e with
+    | Id => neutr
+    | Var v => v
+    | Op e1 e2 => op (expDenote e1) (expDenote e2)
+    | Mor f e' => f (expDenote e')
+    | Inv x => inv (expDenote x)
+end.
+
+Require Import List.
+Import ListNotations.
+
+Fixpoint expDenoteL {X : Grp} (l : list X) : X :=
+match l with
+    | [] => neutr
+    | h :: t => op h (expDenoteL t)
+end.
+
+Fixpoint fib (n : nat) : nat :=
+match n with
+    | 0 => 0
+    | 1 => 1
+    | S (S n' as n'') => (*fib n'' +*) fib n'
+end.
+
+Eval compute in fib 10.
+
+Fixpoint flatten {X : Grp} (e : exp X) {struct e} : list X :=
+match e with
+    | Id => []
+    | Var v => [v]
+    | Op e1 e2 => flatten e1 ++ flatten e2
+    | Mor f Id => []
+    (*| Mor f (Inv e') => *)
+    | Mor f e' => map f (flatten e')
+    (*| Inv (Inv e') => flatten e'*)
+    | Inv e' => rev (map inv (flatten e'))
+end.
+
+Lemma flatten_Hom : forall (X : Grp) (f : GrpHom X X) (e : exp X),
+  e <> Id -> flatten (Mor f e) = map f (flatten e).
+Proof.
+  destruct e; auto.
+Qed.
+
+Lemma flatten_Inv : forall (X : Grp) (e : exp X),
+  (forall e' : exp X, e <> Inv e') ->
+  flatten (Inv e) = rev (map inv (flatten e)).
+Proof.
+  induction e; intros; trivial.
+  (*contradiction (H e). trivial.*)
+Qed.
+
+Lemma expDenoteL_app :
+  forall (X : Grp) (l1 l2 : list X),
+    expDenoteL (l1 ++ l2) == op (expDenoteL l1) (expDenoteL l2).
+Proof.
+  induction l1 as [| h1 t1]; simpl; intros.
+    rewrite neutr_l. reflexivity.
+    rewrite <- assoc. apply op_Proper.
+      reflexivity.
+      rewrite IHt1. reflexivity.
+Qed.
+
+Lemma expDenoteL_hom :
+  forall (X Y : Grp) (f : MonHom X Y) (l : list X),
+    expDenoteL (map f l) == f (expDenoteL l).
+Proof.
+  induction l as [| h t]; simpl.
+    grp.
+    assert (f (op h (expDenoteL t)) == op (f h) (f (expDenoteL t))).
+      grp'.
+      rewrite H. apply op_Proper.
+        reflexivity.
+        assumption.
+Qed.
+
+Lemma inv_Proper : forall (X : Grp), Proper (equiv ==> equiv) inv.
+Proof.
+  unfold Proper, respectful; intros. grpob X.
+  simpl in *. destruct X_inv. simpl in *. f_equiv. assumption.
+Qed.
+
+Lemma expDenoteL_inv :
+  forall (X : Grp) (l : list X),
+    expDenoteL (map inv l) == inv (expDenoteL (rev l)).
+Proof.
+  induction l as [| h t]; simpl.
+    rewrite inv_neutr. reflexivity.
+    assert (inv (op h (expDenoteL t)) == op (inv (expDenoteL t)) (inv h)).
+      rewrite inv_op. reflexivity.
+      pose inv_Proper. rewrite expDenoteL_app. rewrite inv_op. simpl.
+        apply op_Proper.
+          grp.
+          assumption.
+Qed.
+
+Theorem flatten_correct :
+  forall (X : Grp) (e : exp X),
+    expDenoteL (flatten e) == expDenote e.
+Proof.
+  induction e.
+    reflexivity.
+    mon.
+    simpl. rewrite expDenoteL_app. apply op_Proper; assumption.
+    destruct e; simpl; try rewrite expDenoteL_hom; grp.
+    destruct e; simpl in *.
+      rewrite inv_neutr. reflexivity.
+      grp.
+      pose inv_Proper. rewrite <- IHe.
+      rewrite map_app. rewrite rev_app_distr. do 2 rewrite <- map_rev.
+        rewrite expDenoteL_app.
+          replace (flatten e1 ++ flatten e2) with
+            (rev (rev (flatten e1 ++ flatten e2))).
+          rewrite <- expDenoteL_inv. rewrite rev_app_distr.
+            rewrite map_app. rewrite expDenoteL_app. reflexivity.
+          apply rev_involutive.
+      rewrite <- map_rev. rewrite expDenoteL_inv. rewrite rev_involutive.
+        apply inv_Proper. assumption.
+      rewrite <- map_rev. rewrite expDenoteL_inv. apply inv_Proper.
+        rewrite rev_involutive. assumption.
+Qed.
+
+Theorem grp_reflect :
+  forall (X : Grp) (e1 e2 : exp X),
+    expDenoteL (flatten e1) == expDenoteL (flatten e2) ->
+      expDenote e1 == expDenote e2.
+Proof.
+  induction e1; intros; repeat rewrite flatten_correct in H;
+  assumption.
+Qed.
+
+Ltac reify e :=
+lazymatch e with
+    | @neutr ?X => idtac X; constr:(@Id X)
+    | op ?e1 ?e2 =>
+        let e1' := reify e1 in
+        let e2' := reify e2 in constr:(Op e1' e2')
+    | SetoidHom_Fun (SgrHom_Fun (MonHom_SgrHom (GrpHom_MonHom ?f))) ?e =>
+        let e' := reify e in constr:(Mor f e')
+    (*| inv ?e =>
+        let e' := reify e in constr:(Inv e')*)
+    | ?v => constr:(Var v)
+end.
+
+Ltac grp2 := simpl; intros;
+match goal with
+    | |- ?e1 == ?e2 =>
+        let e1' := reify e1 in
+        let e2' := reify e2 in
+          change (expDenote e1' == expDenote e2');
+          apply grp_reflect; simpl
+end.
+
+Ltac grp2' := mon2; try reflexivity.
+
+Goal forall (X : Grp) (a b c : X),
+  op a (op b c) == op (op a b) c.
+Proof.
+  grp2'.
+Qed.
+
+Goal forall (X : Grp) (f : GrpHom X X) (a b : X),
+  f (op a b) == op (f a) (f b).
+Proof.
+  grp2'.
+Qed.
+
+Goal forall (X : Grp) (f : GrpHom X X) (a b c : X),
+  op (f (f neutr)) (op (f a) (f (op b c))) ==
+  op (f a) (op (f b) (f c)).
+Proof.
+  grp2'.
+Qed.
+
+Goal forall (X Y Z : Grp) (f : GrpHom X Y) (g : GrpHom Y Z),
+  g (f neutr) == neutr.
+Proof.
+  intros.
+  let e := reify constr:(@neutr X) in pose e.
+  (* TODO : problem with neutral element. It's argument is Mon,
+     but reify requires it to be Grp. *)
+Qed.
+
 Instance GrpHomSetoid (X Y : Grp) : Setoid (GrpHom X Y) :=
 {
   equiv := fun f g : GrpHom X Y =>
@@ -103,7 +369,7 @@ Proof. apply Setoid_kernel_equiv. Defined.
 Definition GrpComp (X Y Z : Grp) (f : GrpHom X Y) (g : GrpHom Y Z)
     : GrpHom X Z.
 Proof.
-  red. exists (MonComp f g). grp.
+  red. exists (MonComp f g). grp2.
 Defined.
 
 Definition GrpId (X : Grp) : GrpHom X X.
@@ -122,58 +388,6 @@ Proof.
     eapply (@comp_Proper MonCat); auto.
   (* Category laws *) Time all: grp.
 Defined.
-
-Theorem inv_involutive : forall (G : Grp) (g : G),
-    inv (inv g) == g.
-Proof.
-  intros. pose (@op_Proper G).
-  assert (op (inv (inv g)) (op (inv g) g) == g).
-    rewrite assoc, inv_l, neutr_l. reflexivity.
-    rewrite inv_l , neutr_r in H. assumption.
-Qed.
-
-Theorem neutr_unique_l : forall (G : Grp) (e : G),
-    (forall g : G, op e g = g) -> e = neutr.
-Proof.
-  intros. assert (op e neutr = e). grp.
-  assert (op e neutr = neutr). apply H.
-  rewrite H0 in H1. auto.
-Defined.
-
-Theorem neutr_unique_r : forall (G : Grp) (e : G),
-    (forall g : G, op g e = g) -> e = neutr.
-Proof.
-  intros.
-  assert (op neutr e = e). grp.
-  assert (op neutr e = neutr). apply H.
-  rewrite H0 in H1. auto.
-Defined.
-
-Theorem inv_op : forall (G : Grp) (a b : G),
-    inv (op a b) = op (inv b) (inv a).
-Proof.
-  intros. pose (@op_Proper G).
-  assert (forall x y : G, op (op x y) (inv (op x y)) == neutr). auto.
-  assert (forall x y : G, op (op x y) (op (inv y) (inv x)) == neutr).
-    intros. rewrite <- assoc. rewrite (assoc y _). rewrite inv_r.
-    rewrite neutr_l. auto.
-  replace (inv (op a b)) with (op (inv (op a b)) neutr); auto.
-    specialize (H a b).
-    rewrite <- (H0 a b) in H. rewrite inv_r in H.
-      pose (@op_Proper G).
-      (*rewrite H.
-      repeat rewrite <- assoc in H.
-Defined.*)
-(* TODO : group lemmas *)
-
-Theorem inv_neutr : forall (G : Grp), inv neutr = neutr.
-Proof.
-  intros. apply neutr_unique_l. intro.
-  rewrite <- inv_involutive at 1. rewrite inv_op.
-  rewrite inv_involutive. rewrite neutr_r. apply inv_involutive.
-Defined.
-
-Hint Resolve inv_involutive neutr_unique_l neutr_unique_r inv_op inv_neutr.
 
 Instance Grp_zero : Grp :=
 {
